Click.v
@@ -478,6 +478,636 @@ Fixpoint sequence {N} `{Monad N} {A} (l : list (N A)) : N (list A) :=
 
 End Desync.
 
+Arguments well_formed {name}.
+
+Section WF_stage.
+
+  Variable even odd : Set.
+  Context {scheme : naming_scheme even odd}.
+
+  Definition left_env_component (l : latch even odd) :=
+    NOT (ack (latch_input l)) (req (latch_input l)).
+  Definition right_env_component (l : latch even odd) :=
+    forward (req (latch_output l)) (ack (latch_output l)).
+
+
+(*  any click circuit with output ho, input handshake hi:
+    C ⊆ left_env_component ho ∥ right_env_component hi
+
+   l -> l'
+   l -> l''
+
+   latch_stage l = state space with clock l
+   stageMG l = marked graph (as a state space)
+
+    hide l''_in ((stageMG l ∥ fanout l_out l'_in l''_in) ∥ stageMG l')
+    ⊆ stageMG l [l_out ↦ l'_in] ∥ stageMG l'
+
+    if t ∈ hide everything else except local clocks (C ∥ latch_stage l ∥ latch_stage l')
+
+    fanout h h1 h2 ⊆ h ↔ h1 ∥ h ↔ h2
+    then t ∈ (left_env_component ∥ latch_stage l ∥ lout ↔ lin ∥ latch_stage l' ∥ right_env_component)
+    modulo hiding
+
+    and we are proving therefore t ∈ rise_decoupled
+*)
+  Definition latch_stage_with_env l := left_env_component l ∥ latch_stage l ∥ right_env_component l.
+
+
+  Lemma latch_stage_with_env_input : forall l,
+    space_input (latch_stage_with_env l) == ∅.
+  Proof.
+    intros l'. split.
+    2:{ intros x Hx; inversion Hx. }
+    set (Hdisjoint := scheme_all_disjoint l').
+    intros x Hx. simpl in Hx. decompose_set_structure.
+    destruct l'; simpl in *; decompose_set_structure; find_contradiction.
+    destruct l'; simpl in *; decompose_set_structure; find_contradiction.
+  Qed.
+  Lemma latch_stage_with_env_output : forall l,
+    space_output (latch_stage_with_env l) == space_input (latch_stage l) ∪ space_output (latch_stage l).
+  Proof.
+    intros l'.
+    set (Hdisjoint := scheme_all_disjoint l').
+    split.
+    { intros x Hx. simpl in Hx. decompose_set_structure;
+      destruct l'; simpl in *; decompose_set_structure; solve_set.
+    }
+    { intros x Hx. simpl in Hx. decompose_set_structure;
+      destruct l'; simpl in *; decompose_set_structure; solve_set.
+    }
+  Qed.
+  Lemma latch_stage_with_env_internal : forall l,
+    space_internal (latch_stage_with_env l) == space_internal (latch_stage l).
+  Proof.
+    intros l'.
+    set (Hdisjoint := scheme_all_disjoint l').
+    split.
+    { intros x Hx. simpl in Hx. decompose_set_structure;
+      destruct l'; simpl in *; decompose_set_structure; solve_set.
+    }
+    { intros x Hx. simpl in Hx. decompose_set_structure;
+      destruct l'; simpl in *; decompose_set_structure; solve_set.
+    }
+  Qed.
+  Lemma dom_latch_stage_with_env : forall l,
+    space_domain (latch_stage_with_env l) == space_domain (latch_stage l).
+  Proof.
+    intros l'.
+    unfold space_domain.
+    rewrite latch_stage_with_env_input.
+    rewrite latch_stage_with_env_output.
+    rewrite latch_stage_with_env_internal.
+    (* monoid *)
+    admit.
+  Admitted.
+
+
+  Inductive val_is_bit : value -> Prop :=
+  | val_bit0 : val_is_bit Bit0
+  | val_bit1 : val_is_bit Bit1.
+  Lemma val_is_bit_neg_neg : forall v, val_is_bit v -> neg_value (neg_value v) = v.
+  Proof.
+    intros v Hv; inversion Hv; subst; auto.
+  Qed.
+  Lemma val_is_bit_neq : forall v1 v2, val_is_bit v1 -> val_is_bit v2 -> v1 <> v2 -> neg_value v1 = v2.
+  Proof.
+    intros v1 v2 Hv1 Hv2 Hneq;
+      inversion Hv1; inversion Hv2; subst; auto;
+        find_contradiction.
+  Qed.
+  Lemma val_is_bit_neg_inversion : forall v1 v2, val_is_bit v2 ->
+                                                 v1 = neg_value v2 ->
+                                                 neg_value v1 = v2.
+  Proof.
+    intros v1 v2 Hv2 Heq; subst. rewrite val_is_bit_neg_neg; auto.
+  Qed.
+
+  Hint Constructors val_is_bit : click.
+  Inductive wf_handshake (h : handshake) (σ : state name) : Prop :=
+  | handshake_in_sync : σ (req h) = σ (ack h) -> wf_handshake h σ
+  | handshake_out_of_sync : σ (req h) = neg_value (σ (ack h)) -> wf_handshake h σ.
+  Record wf_stage_state (l : latch even odd) (σ : state name) : Prop :=
+    { wf_all_bits : forall x, x ∈ space_domain (latch_stage_with_env l) -> val_is_bit (σ x)
+    ; wf_latch_input  : wf_handshake (latch_input l)  σ
+    ; wf_latch_output : wf_handshake (latch_output l) σ
+    ; wf_ctrl_reset_n : σ (@ctrl_reset_n even odd _) = Bit1
+    }.
+
+  Lemma step_wf_state_σR : forall l,
+    wf_stage_state l (σR l).
+  Proof.
+    intros l.
+    set (Hdisjoint := scheme_all_disjoint l).
+      split.
+      { intros x Hx. unfold σR.
+        repeat (compare_next; try constructor);
+          destruct l; try constructor.
+      }
+      { assert (Hack : σR l (ack (latch_input l)) = Bit0).
+        { unfold σR; reduce_eqb.
+          repeat (compare_next; auto).
+        }
+        assert (Hreq : σR l (req (latch_input l)) = if is_token_latch l then Bit0 else Bit1).
+        { unfold σR; reduce_eqb.
+          repeat (compare_next; auto).
+        }
+        destruct l; simpl in Hreq.
+        * (* Odd==not token latch *)
+          apply handshake_out_of_sync.
+          rewrite Hack, Hreq; auto.
+        * (* Even==token latch *)
+          apply handshake_in_sync.
+          rewrite Hack, Hreq; auto.
+      }
+      { assert (Hack : σR l (ack (latch_output l)) = Bit0).
+        { unfold σR; reduce_eqb; auto. }
+        assert (Hreq : σR l (req (latch_output l)) = if is_token_latch l then Bit1 else Bit0).
+        { unfold σR; reduce_eqb.
+          repeat (compare_next; auto).
+        }
+        destruct l; simpl in Hreq.
+        * (* Odd==not token latch *)
+          apply handshake_in_sync.
+          rewrite Hack, Hreq; auto.
+        * (* Even==token latch *)
+          apply handshake_out_of_sync.
+          rewrite Hack, Hreq; auto.
+      }
+      { unfold σR; reduce_eqb.
+        repeat (compare_next; try constructor);
+          destruct l; try constructor.
+      }
+  Qed.
+
+
+
+
+  Lemma latch_stage_well_formed : forall l, well_formed (latch_stage_with_env l).
+  Proof.
+    intros l.
+    set (Hdisjoint := scheme_all_disjoint l).
+    unfold latch_stage_with_env, left_env_component, right_env_component, latch_stage,
+           latch_stage_with_reset, latch_flop_component.
+    repeat match goal with
+    | [ |- well_formed _] => apply wf_union; auto; try unfold space_domain
+    | [ |- well_formed _ ] => apply hide_wf; auto; simpl; try solve_set
+    | [ |- well_formed _ ] => apply func_wf; solve_set
+    | [ |- in_dec _ ] => simpl; auto 30 with sets; fail
+    | [ |- _ ⊥ _ ] => constructor; intros x Hx; simpl in *; decompose_set_structure; fail
+    end.
+
+    apply flop_wf.
+    destruct l; simpl; repeat (constructor; try_solve_set).
+
+  Qed.
+  Hint Resolve latch_stage_well_formed.
+
+
+Lemma union_inversion_left : forall (S1 S2 : StateSpace name) σ x v σ',
+    (S1 ∥ S2) ⊢ σ →{Some (Event x v)} Some σ' ->
+    x ∈ space_domain S1 ->
+    S1 ⊢ σ →{Some (Event x v)} Some σ'.
+Proof.
+  intros ? ? ? ? ? ? Hstep Hdom.
+  inversion Hstep; subst; auto.
+  (* the only remaining case is when x ∉ dom(S1), a contradiction *)
+  { contradict H0. constructor. auto. }
+Qed.
+
+Lemma union_inversion_right : forall (S1 S2 : StateSpace name) σ x v σ',
+    (S1 ∥ S2) ⊢ σ →{Some (Event x v)} Some σ' ->
+    x ∈ space_domain S2 ->
+    S2 ⊢ σ →{Some (Event x v)} Some σ'.
+Proof.
+  intros ? ? ? ? ? ? Hstep Hdom.
+  inversion Hstep; subst; auto.
+  (* the only remaining case is when x ∉ dom(S2), a contradiction *)
+  { contradict H0. constructor. auto. }
+Qed.
+
+
+
+  Instance internal_in_dec : forall l, in_dec (space_internal (latch_stage_with_env l)).
+  Admitted.
+
+  Instance input_in_dec : forall l, in_dec (space_input (latch_stage_with_env l)).
+  Admitted.
+
+  Instance output_in_dec : forall l, in_dec (space_output (latch_stage_with_env l)).
+  Admitted.
+
+Lemma union_internal_inversion_right : forall (S1 S2 : StateSpace name) σ x v σ',
+    well_formed S1 ->
+    well_formed S2 ->
+    space_internal S1 ⊥ space_domain S2 ->
+    space_domain S1 ⊥ space_internal S2 ->
+    (S1 ∥ S2) ⊢ σ →{ Some (Event x v)} Some σ' ->
+    x ∉ space_domain S2 ->
+    forall y, y ∈ space_internal S2 ->
+    σ' y = σ y.
+Proof.
+  intros ? ? ? ? ? ? Hwf1 Hwf2 Hdisj1 Hdisj2 Hstep Hx y Hy.
+  inversion Hstep; subst; auto.
+  * unfold state_equiv_on in H2.
+    rewrite H2; auto.
+    unfold space_domain; solve_set.
+  * contradict H0.
+    constructor.
+
+    apply wf_space in Hstep; auto.
+    simpl in Hstep.
+    decompose_set_structure; unfold space_domain in *;
+      try solve_set;
+      try (contradict Hx; solve_set).
+      apply wf_union; auto.
+
+  * inversion H0; subst;
+      inversion H4; subst;
+      contradict Hx; unfold space_domain; solve_set.
+
+Qed.
+
+Lemma hide_inversion : forall (S : StateSpace name) σ x e σ',
+    (hide x S) ⊢ σ →{Some e} Some σ' ->
+    S ⊢ σ →{Some e} Some σ'.
+Proof.
+  intros ? ? ? ? ? Hstep.
+  inversion Hstep; auto.
+Qed.
+
+Lemma func_space_output_inversion : forall I (o : name) f (σ : state name) x v σ',
+    o ∉ I ->
+    func_space I o f ⊢ σ →{Some (Event x v)} Some σ' ->
+    x = o ->
+    v = f σ.
+Proof.
+  intros ? ? ? ? ? ? ? Ho Hstep ?. subst.
+    inversion Hstep; try find_contradiction.
+    subst. auto.
+Qed.
+
+Lemma func_space_output_unstable : forall I (o : name) f σ x v σ',
+    o ∉ I ->
+    func_space I o f ⊢ σ →{Some (Event x v)} Some σ' ->
+    x = o ->
+    σ x <> v.
+Proof.
+    intros ? ? ? ? ? ? ? ? Hstep Heq.
+    subst.
+    inversion Hstep; subst; try find_contradiction; auto.
+Qed.
+
+Lemma func_space_output_neq : forall I (o : name) f σ v σ' y,
+    o ∉ I ->
+    func_space I o f ⊢ σ →{Some (Event o v)} Some σ' ->
+    y <> o ->
+    σ' y = σ y.
+Proof.
+  intros ? ? ? ? ? ? ? ? Hstep Hneq.
+  inversion Hstep; subst; unfold update;
+    compare_next; auto.
+Qed.
+
+  Ltac step_inversion_1 :=
+  match goal with
+  | [ Hstep : _ ⊢ _ →{ Some _ } Some _ |- _ ] =>
+      apply union_inversion_left in Hstep;
+          (* the left;right is that we should only succeedd here if x ∈ output(S1) *)
+      [ | unfold space_domain; left; right; simpl; solve_set; fail]
+  | [ Hstep : _ ⊢ _ →{ Some _ } Some _ |- _ ] =>
+      apply union_inversion_right in Hstep;
+          (* the left;right is that we should only succeedd here if x ∈ output(S2) *)
+      [ | unfold space_domain; left; right; simpl; solve_set; fail]
+  | [ Hstep : _ ⊢ _ →{ Some _ } Some _ |- _ ] =>
+      apply hide_inversion in Hstep
+  end.
+  Ltac step_inversion_eq :=
+  repeat step_inversion_1;
+  match goal with
+  | [ Hstep : _ ⊢ _ →{ Some _ } Some _ |- _ ] =>
+      apply func_space_output_inversion in Hstep;
+        [ | simpl; solve_set; fail | simpl; solve_set; fail]
+  end.
+  Ltac step_inversion_unstable :=
+  repeat step_inversion_1;
+  match goal with
+  | [ Hstep : _ ⊢ _ →{ Some _ } Some _ |- _ ] =>
+      eapply func_space_output_unstable in Hstep; eauto;
+        [ | simpl; solve_set; fail ]
+  end.
+
+
+
+
+Ltac rewrite_step_inversion :=
+  match goal with
+    | [ Hstep : latch_stage_with_env ?l ⊢ ?σ →{ Some (Event ?x ?v)} Some ?σ' |- context[ ?σ' ?x ] ] =>
+      rewrite (wf_update _ _ (latch_stage_well_formed l) _ _ _ _ Hstep)
+
+    | [ Hstep : latch_stage_with_env ?l ⊢ ?σ →{ Some (Event ?x ?v)} Some ?σ' |- context[ ?σ' ?y ] ] =>
+      rewrite (wf_scoped _ _ (latch_stage_well_formed l) _ _ _ Hstep);
+        [
+        | intros; inversion 1; find_contradiction
+        | simpl; try (solve_set); try (simpl in *; decompose_set_structure; solve_set); fail ]
+    end.
+
+Ltac solve_wf_handshake :=
+  match goal with
+  | [ H : wf_handshake (?shake ?l) ?σ
+    |- wf_handshake (?shake ?l) _ ] => 
+    inversion H; 
+      try (left;
+        repeat rewrite_step_inversion;
+        step_inversion_eq; auto; fail);
+      try (right;
+        repeat rewrite_step_inversion;
+        step_inversion_eq; auto; fail);
+      fail
+  end.
+
+
+Ltac solve_val_is_bit :=
+  auto;
+  repeat match goal with
+
+  | [ |- context[ latch_to_token_flag ?l ] ] => destruct l; simpl
+
+  | [ Hwf1 : forall x, x ∈ ?X -> val_is_bit (?σ x) |- context[?σ ?y] ] =>
+    let Hwf1' := fresh "Hwf1" in
+    assert (Hwf1' : val_is_bit (σ y))
+      by (apply Hwf1; simpl; try unfold space_domain; solve_set);
+    clear Hwf1;
+    auto
+
+  | [ H : val_is_bit (?σ ?x) |- val_is_bit (?f (?σ ?x)) ] =>
+    inversion H; subst;
+    auto with click
+
+  | [ H : ?S ⊢ ?σ →{Some (Event ?x ?v)} Some ?σ' |- val_is_bit ?v ] =>
+    step_inversion_eq; subst
+
+  | [ |- val_is_bit _ ] =>
+    rewrite_step_inversion
+  end; fail.
+
+
+  Lemma step_wf_state_lemma : forall l σ e σ',
+    wf_stage_state l σ ->
+    latch_stage_with_env l ⊢ σ →{Some e} Some σ' ->
+    wf_stage_state l σ'.
+  Proof.
+    intros l σ [x v] σ' [Hwf1 Hwf2 Hwf3 Hwf4] Hstep.
+    set (Hdisjoint := scheme_all_disjoint l).
+    assert (Hx : x ∈ space_input (latch_stage_with_env l) ∪ space_output (latch_stage_with_env l)).
+    { eapply wf_space; eauto. }
+    rewrite latch_stage_with_env_input, latch_stage_with_env_output in Hx.
+    rewrite latch_stage_input, latch_stage_output in Hx.
+
+    decompose_set_structure;
+    (constructor;
+      [ intros y Hy;
+        match goal with
+        [ Hstep : latch_stage_with_env ?l ⊢ ?σ →{ Some (Event ?x _)} Some ?σ' |- _] =>
+          compare y x; try solve_val_is_bit
+        end
+      | try solve_wf_handshake
+      | try solve_wf_handshake
+      | try solve_val_is_bit
+      ]).
+
+    *
+      destruct (y ∈? space_internal (latch_stage_with_env l)) as [Hinternal | Hinternal].
+      2:{
+        rewrite (wf_scoped _ _ (latch_stage_well_formed l) _ _ _ Hstep);
+        [
+        | intros; inversion 1; find_contradiction
+        | simpl; try (solve_set); try (simpl in *; decompose_set_structure; solve_set) ].
+        solve_val_is_bit.
+      }
+      1:{
+        (* when req (latch_input l) event occurs, no internal wires change... *)
+        assert (Heq : σ' y = σ y).
+        { repeat step_inversion_1.
+          eapply func_space_output_neq; [ | eauto | ]; solve_set.
+        }
+        rewrite Heq. solve_val_is_bit.
+      }
+
+    * (* ctrl_reset_n *)
+      repeat step_inversion_1.
+      (* rewrite_step_inversion ??? *)
+      erewrite (wf_scoped _ _ _ _ _ _ Hstep).
+      2:{ intros. inversion 1; find_contradiction. }
+      2:{ simpl. solve_set. }
+      auto.
+
+    * (* ack (latch_output l) *)
+      destruct (y ∈? space_internal (latch_stage_with_env l)) as [Hinternal | Hinternal].
+      + assert (Heq : σ' y = σ y).
+        { repeat step_inversion_1.
+          eapply func_space_output_neq; [ | eauto | ]; solve_set.
+        }
+        rewrite Heq. solve_val_is_bit.
+      + rewrite (wf_scoped _ _ (latch_stage_well_formed l) _ _ _ Hstep);
+        [
+        | intros; inversion 1; find_contradiction
+        | simpl; try (solve_set); try (simpl in *; decompose_set_structure; solve_set); fail ].
+        solve_val_is_bit.
+
+    * (* ctrl_reset_n *)
+      repeat step_inversion_1.
+      (* rewrite_step_inversion ??? *)
+      erewrite (wf_scoped _ _ _ _ _ _ Hstep).
+      2:{ intros. inversion 1; find_contradiction. }
+      2:{ simpl. solve_set. }
+      auto.
+
+    * (* ack (latch_input l) *)
+      destruct (y ∈? space_internal (latch_stage_with_env l)) as [Hinternal | Hinternal].
+      + assert (Heq : σ' y = σ y).
+        { repeat step_inversion_1.
+          eapply func_space_output_neq; [ | eauto | ]; solve_set.
+        }
+        rewrite Heq. solve_val_is_bit.
+      + rewrite (wf_scoped _ _ (latch_stage_well_formed l) _ _ _ Hstep);
+        [
+        | intros; inversion 1; find_contradiction
+        | simpl; try (solve_set); try (simpl in *; decompose_set_structure; solve_set); fail ].
+        solve_val_is_bit.
+
+
+
+    * assert (Hstate0' :
+                σ (ack (latch_input l)) = match latch_to_token_flag l with
+                           | Token => σ (latch_state0 l)
+                           | NonToken => neg_value (σ (latch_state0 l))
+                           end).
+       { assert (v_bit : val_is_bit v).
+         { step_inversion_eq; subst. solve_val_is_bit. }
+         assert (Hneq : σ (ack (latch_input l)) = neg_value v).
+         { step_inversion_unstable.
+           erewrite val_is_bit_neq; eauto.
+           solve_val_is_bit.
+         }
+
+         replace v with
+            (match latch_to_token_flag l with
+             | Token => neg_value (σ (latch_state0 l))
+             | NonToken => σ (latch_state0 l)
+             end) in * by (step_inversion_eq; auto).
+         rewrite Hneq.
+         destruct l; simpl; auto.
+         rewrite val_is_bit_neg_neg; auto; solve_val_is_bit.
+       }
+        inversion Hwf2.
+        + right. repeat rewrite_step_inversion.
+          step_inversion_eq. subst.
+          rewrite H0.
+          rewrite Hstate0'.
+          destruct l; simpl; auto.
+
+
+          rewrite val_is_bit_neg_neg; auto. solve_val_is_bit.
+
+        + left. repeat rewrite_step_inversion.
+          step_inversion_eq. subst.
+          rewrite H0.
+          rewrite Hstate0'.
+          destruct l; simpl; auto.
+
+          rewrite val_is_bit_neg_neg; auto. solve_val_is_bit.
+
+    * (* ctrl_reset_n *)
+      repeat step_inversion_1.
+      (* rewrite_step_inversion ??? *)
+      erewrite (wf_scoped _ _ _ _ _ _ Hstep).
+      2:{ intros. inversion 1; find_contradiction. }
+      2:{ simpl. solve_set. }
+      auto.
+
+    * (* req (latch_output l) *)
+      destruct (y ∈? space_internal (latch_stage_with_env l)) as [Hinternal | Hinternal].
+      + assert (Heq : σ' y = σ y).
+        { repeat step_inversion_1.
+          eapply func_space_output_neq; [ | eauto | ]; solve_set.
+        }
+        rewrite Heq. solve_val_is_bit.
+      + rewrite (wf_scoped _ _ (latch_stage_well_formed l) _ _ _ Hstep);
+        [
+        | intros; inversion 1; find_contradiction
+        | simpl; try (solve_set); try (simpl in *; decompose_set_structure; solve_set); fail ].
+        solve_val_is_bit.
+
+    * assert (Hstate0 : σ (req (latch_output l)) = neg_value (σ (latch_state0 l))).
+      { replace v with (σ (latch_state0 l)) in * by (step_inversion_eq; auto).
+        step_inversion_unstable.
+        erewrite val_is_bit_neq; eauto; solve_val_is_bit.
+      }
+
+      inversion Hwf3.
+        + right. repeat rewrite_step_inversion.
+          step_inversion_eq. subst.
+          rewrite <- H0.
+          rewrite Hstate0.
+          rewrite val_is_bit_neg_neg; auto. solve_val_is_bit.
+
+        + left. repeat rewrite_step_inversion.
+          step_inversion_eq. subst.
+
+
+      apply val_is_bit_neg_inversion in H0; try solve_val_is_bit.
+      rewrite <- H0.
+      rewrite Hstate0.
+      rewrite val_is_bit_neg_neg; auto; solve_val_is_bit.
+
+    * (* ctrl_reset_n *)
+      repeat step_inversion_1.
+      (* rewrite_step_inversion ??? *)
+      erewrite (wf_scoped _ _ _ _ _ _ Hstep).
+      2:{ intros. inversion 1; find_contradiction. }
+      2:{ simpl. solve_set. }
+      auto.
+
+    * (* latch_clk *)
+      rewrite_step_inversion.
+      step_inversion_eq; subst.
+      unfold tok_clk_defn, clk_defn.
+      assert (Hctrl : σ (@ctrl_reset_n _ _ scheme) = Num 1) by admit (* why?? *).
+      assert (Hreq : val_is_bit (σ (req (latch_input l))))
+        by (apply Hwf1; simpl; try unfold space_domain; solve_set).
+      assert (Hack : val_is_bit (σ (ack (latch_output l))))
+        by (apply Hwf1; simpl; try unfold space_domain; solve_set).
+      assert (Hstate0 : val_is_bit (σ (latch_state0 l)))
+        by (apply Hwf1; simpl; try unfold space_domain; solve_set).
+
+      destruct l; simpl; rewrite Hctrl;
+        inversion Hreq; subst; simpl;
+        inversion Hstate0; subst; simpl;
+        inversion Hack; subst; simpl; constructor.
+
+    * (* latch_clk *)
+      destruct (y ∈? space_internal (latch_stage_with_env l)) as [Hinternal | Hinternal].
+      + assert (Heq : σ' y = σ y).
+        { repeat step_inversion_1.
+          eapply func_space_output_neq; [ | eauto | ]; solve_set.
+        }
+        rewrite Heq. solve_val_is_bit.
+      + rewrite (wf_scoped _ _ (latch_stage_well_formed l) _ _ _ Hstep);
+        [
+        | intros; inversion 1; find_contradiction
+        | simpl; try (solve_set); try (simpl in *; decompose_set_structure; solve_set); fail ].
+        solve_val_is_bit.
+
+    * (* ctrl_reset_n *)
+      repeat step_inversion_1.
+      (* rewrite_step_inversion ??? *)
+      erewrite (wf_scoped _ _ _ _ _ _ Hstep).
+      2:{ intros. inversion 1; find_contradiction. }
+      2:{ simpl. solve_set. }
+      auto.
+
+(*
+    * (* latch_clk *)
+      rewrite_step_inversion.
+      step_inversion_eq; subst.
+      unfold tok_clk_defn, clk_defn.
+      assert (Hctrl : σ (@ctrl_reset_n _ _ scheme) = Num 1) by admit (* why?? *).
+      assert (Hreq : val_is_bit (σ (req (latch_input l))))
+        by (apply Hwf1; simpl; try unfold space_domain; solve_set).
+      assert (Hack : val_is_bit (σ (ack (latch_output l))))
+        by (apply Hwf1; simpl; try unfold space_domain; solve_set).
+      assert (Hstate0 : val_is_bit (σ (latch_state0 l)))
+        by (apply Hwf1; simpl; try unfold space_domain; solve_set).
+
+      destruct l; simpl; rewrite Hctrl;
+        inversion Hreq; subst; simpl;
+        inversion Hstate0; subst; simpl;
+        inversion Hack; subst; simpl; constructor.
+*)
+  Admitted.
+
+
+  Lemma step_wf_state_eps : forall l σ σ',
+    wf_stage_state l σ ->
+    latch_stage_with_env l ⊢ σ →{None} Some σ' ->
+    wf_stage_state l σ'.
+  Admitted.
+  Lemma step_wf_state : forall l tr σ,
+    latch_stage_with_env l ⊢ σR l →*{tr} Some σ ->
+    wf_stage_state l σ.
+  Proof.
+    intros l tr σ Hstep.
+    set (Hdisjoint := scheme_all_disjoint l).
+    remember (Some σ) as τ; generalize dependent σ.
+    induction Hstep; intros σ Hτ; subst.
+    * inversion Hτ; subst.
+      apply step_wf_state_σR.
+    * eapply step_wf_state_lemma; eauto.
+    * eapply step_wf_state_eps; eauto.
+  Qed.
+
+End WF_stage.
 End Click.
 
 Arguments latch_input  {name even odd} {naming_scheme}.
